src/bst.v
@@ -1,6 +1,6 @@
 From Equations Require Import Equations.
 From Coq Require Import ssreflect ssrbool ssrfun.
-From mathcomp Require Import eqtype ssrnat seq order path.
+From mathcomp Require Import eqtype choice ssrnat seq order path.
 From favssr Require Import prelude bintree.
 Set Implicit Arguments.
 Unset Strict Implicit.
@@ -93,7 +93,7 @@ Lemma inorder_split_min (l r t : tree T) a x :
 Proof.
 elim: l a r t=>/=; first by move=>a r t; case=>->->.
 move=>ll IHl al rl _ a r t.
-case Hsm: (split_min ll al rl)=>[x0 l'] [Hx <-] /=.
+case Hsm: (split_min ll al rl)=>[x0 l'][Hx <-] /=.
 rewrite {}Hx in Hsm; rewrite -cat_cons.
 by rewrite (IHl _ _ _ Hsm).
 Qed.
@@ -224,7 +224,7 @@ End Correctness.
 Section CorrectnessProofs.
 Context {disp : unit} {T : orderType disp}.
 
-Definition bst_list (t : tree T) : bool := sorted <%O (inorder t).
+(* sorted list library *)
 
 Fixpoint ins_list (x : T) (xs : seq T) : seq T :=
   if xs is a::xs' then
@@ -240,12 +240,69 @@ Fixpoint del_list (x : T) (xs : seq T) : seq T :=
       else a :: del_list x xs'
   else [::].
 
+Lemma inorder_ins_list x xs :
+  sorted <%O xs ->
+  perm_eq (ins_list x xs)
+          (if x \in xs then xs else x :: xs).
+Proof.
+elim: xs=>//=a xs IH Hp.
+case: ifP.
+- move/[dup]=>Hxa; rewrite inE lt_neqAle => /andP [/negbTE -> _] /=.
+  move: IH; case: ifP=>//.
+  move: (order_path_min lt_trans Hp) => /allP /[apply] Hax.
+  by move: (lt_asym x a); rewrite Hxa Hax.
+move/negbT; rewrite inE -leNgt=>Hax; case: ifP=>//=.
+move/negbT=>Hxa; move/path_sorted: Hp=>/IH.
+case: ifP=>H; first by rewrite perm_cons.
+by move=>H1; rewrite perm_sym -cat1s -(cat1s a) perm_catCA /= perm_cons perm_sym.
+Qed.
+
+Lemma ins_list_sorted x xs :
+  sorted <%O xs -> sorted <%O (ins_list x xs).
+Proof.
+elim: xs=>//=a xs IH H.
+case: ifP=>/=; first by move=>->.
+move/negbT; rewrite -leNgt=>Hax.
+case: ifP=>//= Hxa.
+move: Hax; rewrite le_eqVlt eq_sym Hxa /= => {Hxa}Hax.
+move/path_sorted: (H)=>/[dup] Hs /IH H'.
+rewrite path_min_sorted {H'}//.
+move: (order_path_min lt_trans H)=>Ha.
+rewrite (perm_all _ (inorder_ins_list _ Hs)); case: ifP=>//= _.
+by rewrite Hax.
+Qed.
+
 Lemma del_nop y xs :
   path <%O y xs -> del_list y xs = xs.
 Proof.
 elim: xs=>//=x xs IH /andP [H1 H2].
 move: (H1); rewrite lt_neqAle=>/andP [/negbTE -> _].
 by rewrite IH //; apply/(path_le lt_trans)/H2.
+Qed.
+
+Lemma inorder_del_list x xs :
+  sorted <%O xs ->
+  perm_eq (del_list x xs)
+          (filter (predC1 x) xs).
+Proof.
+elim: xs=>//=a xs IH Hp.
+move/path_sorted: (Hp)=>/IH {IH}H.
+case: ifP.
+- move/eqP=>E; move: H; rewrite E eq_refl /=.
+  by apply/perm_trans; rewrite perm_sym del_nop.
+by move/negbT=>Hx; rewrite eq_sym Hx perm_cons.
+Qed.
+
+Lemma del_list_sorted x xs :
+  sorted <%O xs -> sorted <%O (del_list x xs).
+Proof.
+elim: xs=>//=a xs IH H.
+move/path_sorted: (H)=>/[dup] H1 /IH {IH}H2.
+case: ifP=>//= /negbT Hxa.
+rewrite path_min_sorted //.
+move: (order_path_min lt_trans H)=>Ha.
+rewrite (perm_all _ (inorder_del_list _ H1)) all_filter.
+by apply/sub_all/Ha=>z /= ->; exact: implybT.
 Qed.
 
 Lemma sorted_cat_cons_cat (l r : seq T) x :
@@ -270,13 +327,13 @@ rewrite all_cat /= andbT => /andP [Hxs Hya].
 case: ifP.
 - move=>Ha; case: ifP=>// /negbT Hy.
   move=>IH; case: ifP=>//= /negbT He.
-  by rewrite IH // -(path_min_sorted (x:=y)) // all_cat /= Hxs Hya.
+  by rewrite IH //; apply: (path_sorted H).
 move=>/negbT Ha; case: ifP; first by move=>Ha'; rewrite Ha' in Ha.
 move=>_; case: ifP.
 - move/eqP=>{Ha}->; case: ifP=>/=.
   - by rewrite ltNge le_eqVlt Hya orbT.
-  move/negbT; rewrite -leNgt=>_; case: ifP=>// _ IH.
-  by rewrite IH // -(path_min_sorted (x:=y)) // all_cat /= andbT Hxs Hya.
+  move/negbT; rewrite -leNgt=>_; case: ifP=>// _.
+  by move=>->//; apply: (path_sorted H).
 move/negbT=>Ha'; move: Ha; rewrite lt_neqAle Ha' /= -ltNge=>{Ha'}Hx.
 case: ifP.
 - move=>Hy _; move: (lt_trans Hy Hya).
@@ -284,7 +341,7 @@ case: ifP.
 move/negbT=>Hy; case: ifP.
 - move/eqP=>He; rewrite He in Hx; move: Hx.
   by rewrite ltNge le_eqVlt Hya orbT.
-by move/eqP=>He IH; rewrite IH // -(path_min_sorted (x:=y)) // all_cat /= Hxs Hya.
+by move/eqP=>_ ->//; apply: (path_sorted H).
 Qed.
 
 Lemma dellist_sorted_cat_cons_cat (xs ys : seq T) x a :
@@ -302,17 +359,21 @@ move: (H); move/(order_path_min lt_trans).
 rewrite all_cat /= => /and3P [Hxs Hya Hys].
 case: ifP.
 - move=>Ha; case: ifP=>// /negbT Hy.
-  by move=>IH; rewrite IH // -(path_min_sorted (x:=y)) // all_cat /= Hxs Hya.
+  by move=>-> //; apply: (path_sorted H).
 move=>/negbT Ha; case: ifP.
 - move/eqP=>{Ha}->; case: ifP=>/=.
   - by move/eqP=>Hay; rewrite Hay ltxx in Hya.
-  by move=>_ IH; rewrite IH // -(path_min_sorted (x:=y)) // all_cat /= Hxs Hya.
+  by move=>_ ->//; apply: (path_sorted H).
 move/negbT=>Ha'; move: Ha; rewrite lt_neqAle Ha' /= -ltNge=>{Ha'}Hx.
 case: ifP.
 - move/eqP=>He; rewrite He in Hx; move: Hx.
   by rewrite ltNge le_eqVlt Hya orbT.
-by move/negbT=>Hxy IH; rewrite IH // -(path_min_sorted (x:=y)) // all_cat /= Hxs Hya.
+by move/negbT=>_ -> //; apply: (path_sorted H).
 Qed.
+
+(* BST via sorted lists *)
+
+Definition bst_list (t : tree T) : bool := sorted <%O (inorder t).
 
 Lemma inorder_insert_list x t :
   bst_list t ->
@@ -380,4 +441,367 @@ case/andP=>+ _ => /allP/(_ z)/[apply] Hz.
 by move: (lt_trans Hz Hx); rewrite lt_neqAle eq_sym=>/andP [/negbTE].
 Qed.
 
+Corollary inorder_insert_list_set x (t : tree T) :
+  bst_list t ->
+  perm_eq (inorder (insert x t))
+          (if x \in inorder t then inorder t else x :: inorder t).
+Proof.
+rewrite /bst_list => Hn.
+rewrite inorder_insert_list //.
+by apply: inorder_ins_list.
+Qed.
+
+Corollary inorder_delete_list_set x (t : tree T) :
+  bst_list t ->
+  perm_eq (inorder (delete x t))
+          (filter (predC1 x) (inorder t)).
+Proof.
+rewrite /bst_list => Hn.
+rewrite inorder_delete_list //.
+by apply: inorder_del_list.
+Qed.
+
+Corollary bst_list_empty : bst_list (@empty _ T).
+Proof. by []. Qed.
+
+Corollary bst_list_insert x (t : tree T) :
+  bst_list t -> bst_list (insert x t).
+Proof.
+move=>H; rewrite /bst_list inorder_insert_list //.
+by apply: ins_list_sorted.
+Qed.
+
+Corollary bst_list_delete x (t : tree T) :
+  bst_list t -> bst_list (delete x t).
+Proof.
+move=>H; rewrite /bst_list inorder_delete_list //.
+by apply: del_list_sorted.
+Qed.
+
 End CorrectnessProofs.
+
+Section IntervalTrees.
+Context {disp : unit} {T : orderType disp}.
+
+(* intervals *)
+
+Structure ivl : Type := Interval {ival :> T * T; _ : ival.1 <= ival.2}.
+
+Canonical interval_subType := Eval hnf in [subType for ival].
+
+Definition interval_eqMixin := Eval hnf in [eqMixin of ivl by <:].
+Canonical interval_eqType := Eval hnf in EqType ivl interval_eqMixin.
+Definition interval_choiceMixin := [choiceMixin of ivl by <:].
+Canonical interval_choiceType := Eval hnf in ChoiceType ivl interval_choiceMixin.
+
+Definition low: ivl -> T := fst \o ival.
+Definition high: ivl -> T := snd \o ival.
+
+Lemma xivl_eqE x y : (x == y) = (low x == low y) && (high x == high y).
+Proof.
+by rewrite /low /high -val_eqE
+  (surjective_pairing (val x)) (surjective_pairing (val y)) xpair_eqE.
+Qed.
+
+Definition lt_ivl x y := (low x < low y) || (low x == low y) && (high x < high y).
+Definition le_ivl x y := (low x < low y) || (low x == low y) && (high x <= high y).
+
+Fact lt_def_ivl : forall x y, lt_ivl x y = (y != x) && (le_ivl x y).
+Proof.
+move=>x y; rewrite /lt_ivl /le_ivl.
+case H: (y==x)=>/=.
+- by move/eqP: H=>->; rewrite !ltxx andbF.
+suff: (low x != low y) || (high x != high y).
+- case/orP; first by move/negbTE=>->.
+  by rewrite (lt_neqAle (high _))=>->.
+move/negbT: H; rewrite -negb_and; apply: contra.
+by rewrite -xivl_eqE eq_sym.
+Qed.
+
+Fact refl_ivl : reflexive le_ivl.
+Proof. by move=>x; rewrite /le_ivl ltxx eq_refl lexx. Qed.
+
+Fact anti_ivl : antisymmetric le_ivl.
+Proof.
+move=>x y; rewrite /le_ivl => /andP [].
+case/orP=>[H1|/andP [/eqP H11 H21]]; case/orP=>[H2|/andP [/eqP H12 H22]].
+- by move: (lt_asym (low x) (low y)); rewrite H1 H2.
+- by rewrite H12 ltxx in H1.
+- by rewrite H11 ltxx in H2.
+apply/val_inj.
+move: {H12}H11 H21 H22; case: x =>[[x1 x2] /= Hx]; case: y =>[[y1 y2] /= Hy].
+rewrite /low /high /= => -> H1 H2.
+by move: (eq_le x2 y2); rewrite H1 H2 /= => /eqP ->.
+Qed.
+
+Fact trans_ivl : transitive le_ivl.
+Proof.
+move=>x y z; rewrite /le_ivl.
+case/orP=>[H1|/andP [/eqP H11 H21]]; case/orP=>[H2|/andP [/eqP H12 H22]].
+- by move: (lt_trans H1 H2)=>->.
+- by rewrite -H12 H1.
+- by rewrite H11 H2.
+rewrite H11 H12 ltxx eq_refl /=.
+by apply/le_trans/H22.
+Qed.
+
+Definition ivl_porderMixin : lePOrderMixin interval_eqType :=
+  LePOrderMixin lt_def_ivl refl_ivl anti_ivl trans_ivl.
+Canonical ivl_porderType := Eval hnf in POrderType tt ivl ivl_porderMixin.
+
+Fact total_ivl : total le_ivl.
+Proof.
+move=>x y; rewrite /le_ivl.
+case: (ltgtP (low x) (low y))=>//= _.
+by apply: le_total.
+Qed.
+
+Definition ivl_totalPOrderMixin :
+  totalPOrderMixin ivl_porderType := total_ivl.
+Canonical multinom_latticeType :=
+  Eval hnf in LatticeType ivl ivl_totalPOrderMixin.
+Canonical ivl_distrLatticeType :=
+  Eval hnf in DistrLatticeType ivl ivl_totalPOrderMixin.
+Canonical ivl_orderType :=
+  Eval hnf in OrderType ivl ivl_totalPOrderMixin.
+
+Definition overlap (x y : ivl) := (low y <= high x) && (low x <= high y).
+
+Lemma overlapC x y : overlap x y = overlap y x.
+Proof. by rewrite /overlap andbC. Qed.
+
+Definition has_overlap (s : seq ivl) y := has (overlap^~ y) s.
+
+(* interval trees = trees of intervals augmented with maximal values *)
+
+Fixpoint isin_a {A} (t : tree (T*A)) x : bool :=
+  if t is Node l (a,_) r
+    then match cmp x a with
+           | LT => isin_a l x
+           | EQ => true
+           | GT => isin_a r x
+         end
+  else false.
+
+Definition ivl_tree := tree (ivl * T).
+
+(* TODO construct a proper bLattice? *)
+Variables (x0 : T) (lmin : left_id x0 Order.max).
+
+Lemma rmin : right_id x0 Order.max.
+Proof. by move=>x; rewrite maxC lmin. Qed.
+
+Definition max3 (m : T) (a : ivl) (n : T) : T :=
+  Order.max (high a) (Order.max m n).
+
+Definition max_hi : ivl_tree -> T := b_val x0.
+
+Definition inv_max_hi : ivl_tree -> bool := invar_f x0 max3.
+
+Lemma max_hi_max t x :
+  inv_max_hi t -> x \in inorder_a t -> high x <= max_hi t.
+Proof.
+elim: t=>/=; first by rewrite in_nil.
+move=>l IHl [a m] r IHr /and3P [/eqP -> /IHl Hl /IHr Hr] {IHl IHr}.
+rewrite mem_cat inE /max3; case/or3P.
+- move/Hl=>H.
+  apply/(le_trans H)/(le_trans (y:=Order.max (max_hi l) (max_hi r)));
+  by rewrite le_maxr lexx ?orbT.
+- by move/eqP=>->; rewrite le_maxr lexx.
+move/Hr=>H.
+apply/(le_trans H)/(le_trans (y:=Order.max (max_hi l) (max_hi r)));
+by rewrite le_maxr lexx ?orbT.
+Qed.
+
+Lemma max_hi_mem t :
+  inv_max_hi t -> is_node t ->
+  has (fun a => high a == max_hi t) (inorder_a t).
+Proof.
+elim: t=>//= l IHl [a m] r IHr /and3P [/eqP E /IHl Hl /IHr Hr] {IHl IHr} _.
+rewrite has_cat /=.
+case: r E Hr=>/=; case: l Hl=>/=; rewrite /max3.
+- by move=>_ + _; rewrite lmin rmin =>->; rewrite eq_refl.
+- move=>ll [al ml] lr H; rewrite orbF rmin /Order.max; case: ifP=>_ -> _;
+  by rewrite ?H // eq_refl orbT.
+- move=>_ rl [ar mr] rr; rewrite lmin /Order.max=>+ H; case: ifP=>_ ->;
+  by rewrite ?eq_refl // H // orbT.
+move=>ll [al ml] lr Hl rl [ar mr] rr; rewrite /Order.max; case: ifP=>_.
+- case: ifP=>_-> Hr; last by rewrite Hl.
+  by rewrite Hr // !orbT.
+by move=>->_; rewrite eq_refl /= orbT.
+Qed.
+
+(* sets of intervals *)
+
+Definition node_i : ivl_tree -> ivl -> ivl_tree -> ivl_tree :=
+  node_f x0 max3.
+
+Fixpoint insert_i x (t : ivl_tree) : ivl_tree :=
+  if t is Node l (a,m) r
+    then match cmp x a with
+           | LT => node_i (insert_i x l) a r
+           | EQ => Node l (a,m) r
+           | GT => node_i l a (insert_i x r)
+         end
+  else Node (@Leaf (ivl*T)) (x, high x) (@Leaf (ivl*T)).
+
+Fixpoint split_min_i (l : ivl_tree) (a : ivl) (r : ivl_tree) : ivl * ivl_tree :=
+  if l is Node ll (al, _) rl then
+    let '(x, l') := split_min_i ll al rl in
+        (x, node_i l' a r)
+    else (a, r).
+
+Lemma inorder_ivl_split_min (l r t : ivl_tree) a x :
+  split_min_i l a r = (x, t) ->
+  x :: inorder_a t = inorder_a l ++ a :: inorder_a r.
+Proof.
+elim: l a r t=>/=; first by move=>a r t; case=>->->.
+move=>ll IHl [al _] rl _ a r t.
+case Hsm: (split_min_i ll al rl)=>[x' l'][Hx <-] /=.
+rewrite {}Hx in Hsm; rewrite -cat_cons.
+by rewrite (IHl _ _ _ Hsm).
+Qed.
+
+Fixpoint delete_i x (t : ivl_tree) : ivl_tree :=
+  if t is Node l (a,_) r
+    then match cmp x a with
+           | LT => node_i (delete_i x l) a r
+           | EQ => if r is Node lr (ar,_) rr
+                     then let '(a', r') := split_min_i lr ar rr in
+                          node_i l a' r'
+                     else l
+           | GT => node_i l a (delete_i x r)
+         end
+  else @Leaf (ivl*T).
+
+(* functional correctness *)
+
+Lemma inorder_ivl_insert_list x t :
+  sorted <%O (inorder_a t) ->
+  inorder_a (insert_i x t ) = ins_list x (inorder_a t).
+Proof.
+elim: t=>//=l IHl [a m] r IHr.
+rewrite sorted_cat_cons_cat=>/andP [H1 H2].
+rewrite inslist_sorted_cat_cons_cat //.
+case Hc: (cmp x a)=>/=.
+- move/cmp_lt: Hc=>->; rewrite IHl //.
+  by rewrite (cat_sorted2 H1).
+- by move/cmp_eq: Hc=>/eqP ->; rewrite ltxx eq_refl.
+move/cmp_gt: Hc=>/[dup] Hx.
+rewrite ltNge le_eqVlt negb_or=>/andP [/negbTE -> /negbTE ->].
+rewrite IHr //.
+by rewrite -cat1s in H2; rewrite (cat_sorted2 H2).
+Qed.
+
+Lemma inorder_ivl_delete_list x t :
+  sorted <%O (inorder_a t) ->
+  inorder_a (delete_i x t) = del_list x (inorder_a t).
+Proof.
+elim: t=>//=l IHl [a m] r IHr /[dup] H.
+rewrite sorted_cat_cons_cat=>/andP [H1 H2].
+rewrite dellist_sorted_cat_cons_cat //.
+case Hc: (cmp x a)=>/=.
+- move/cmp_lt: Hc=>->; rewrite IHl //.
+  by rewrite (cat_sorted2 H1).
+- move/cmp_eq: Hc=>/eqP ->; rewrite ltxx eq_refl.
+  case: {IHr H H2}r=>//=; first by rewrite cats0.
+  move=>lr [ar _] rr.
+  case Hsm: (split_min_i lr ar rr)=>[x' l'] /=.
+  by rewrite (inorder_ivl_split_min Hsm).
+move/cmp_gt: Hc=>/[dup] Hx.
+rewrite ltNge le_eqVlt negb_or=>/andP [/negbTE -> /negbTE ->].
+rewrite IHr //.
+by rewrite -cat1s in H2; rewrite (cat_sorted2 H2).
+Qed.
+
+Lemma inv_max_hi_insert x t :
+  inv_max_hi t -> inv_max_hi (insert_i x t).
+Proof.
+elim: t=>/=; first by rewrite /max3 lmin rmin eq_refl.
+move=>l IHl [a m] r IHr /and3P [/eqP E Hl Hr].
+move:(IHl Hl)=>{}IHl; move:(IHr Hr)=>{}IHr.
+case: (cmp x a)=>/=.
+- by rewrite eq_refl IHl Hr.
+- by rewrite E eq_refl Hl Hr.
+by rewrite eq_refl Hl IHr.
+Qed.
+
+Lemma inv_max_split_min (l r t : ivl_tree) a x :
+  split_min_i l a r = (x, t) ->
+  inv_max_hi l -> inv_max_hi r ->
+  inv_max_hi t.
+Proof.
+elim: l a r t=>/=.
+- by move=>a r t; case=>_->.
+move=>ll IHl [al ml] rl _ a r t.
+case Hsm: (split_min_i ll al rl)=>[x' l'] [Hx <-] /=; rewrite {}Hx in Hsm.
+case/and3P=>He Hll Hrl Har.
+rewrite eq_refl Har /= andbT.
+by rewrite (IHl _ _ _ Hsm Hll Hrl).
+Qed.
+
+Lemma inv_max_hi_delete x t :
+  inv_max_hi t -> inv_max_hi (delete_i x t).
+Proof.
+elim: t=>//=.
+move=>l IHl [a m] r IHr /and3P [/eqP E Hl Hr].
+move:(IHl Hl)=>{}IHl; move:(IHr Hr)=>{}IHr.
+case: (cmp x a)=>/=.
+- by rewrite eq_refl IHl Hr.
+- case: {E IHr}r Hr=>//= lr [ar mr] rr.
+  case/and3P=>_ Hlr Hrr.
+  case Hsm: (split_min_i lr ar rr)=>[x' l'] /=.
+  by rewrite eq_refl Hl /=; apply: (inv_max_split_min Hsm).
+by rewrite eq_refl Hl IHr.
+Qed.
+
+(* top-level correctness *)
+
+Definition invar t := inv_max_hi t && sorted <%O (inorder_a t).
+
+Corollary inorder_ivl_insert_list_set x (t : ivl_tree) :
+  invar t ->
+  perm_eq (inorder_a (insert_i x t))
+          (if x \in inorder_a t then inorder_a t else x :: inorder_a t).
+Proof.
+rewrite /invar => /andP [_ Hs].
+rewrite inorder_ivl_insert_list //.
+by apply: inorder_ins_list.
+Qed.
+
+Corollary inorder_ivl_delete_list_set x (t : ivl_tree) :
+  invar t ->
+  perm_eq (inorder_a (delete_i x t))
+          (filter (predC1 x) (inorder_a t)).
+Proof.
+rewrite /invar => /andP [_ Hs].
+rewrite inorder_ivl_delete_list //.
+by apply: inorder_del_list.
+Qed.
+
+Corollary invar_insert x (t : ivl_tree) :
+  invar t -> invar (insert_i x t).
+Proof.
+rewrite /invar => /andP [Hi Hs].
+rewrite inv_max_hi_insert //= inorder_ivl_insert_list //.
+by apply: ins_list_sorted.
+Qed.
+
+Corollary invar_delete x (t : ivl_tree) :
+  invar t -> invar (delete_i x t).
+Proof.
+rewrite /invar => /andP [Hi Hs].
+rewrite inv_max_hi_delete //= inorder_ivl_delete_list //.
+by apply: del_list_sorted.
+Qed.
+
+(* searching for an overlapping interval *)
+
+Fixpoint search (t : ivl_tree) (x : ivl) : bool :=
+  if t is Node l (a,_) r then
+    if overlap x a then true
+      else if is_node l && (low x <= max_hi l)
+        then search l x else search r x
+    else false.
+
+End IntervalTrees.
